final project/ForWhileEquiv.v
@@ -1,0 +1,107 @@
+(**
+*  CS386L Programming Languages
+* Final project
+* Tian Zhang (tz3272)
+* Brief Introduction:
+*     For the this file, I am working on for while loop equivalence, and 
+      all the work is based on Maps, Imp in class. I got some idea from
+      the book
+*)
+
+Require Import ProgramEquivalence.
+Require Import Coq.Bool.Bool.
+Require Import Coq.Arith.Arith.
+Require Import Coq.Arith.EqNat.
+Require Import Coq.omega.Omega.
+Require Import Coq.Lists.List.
+Require Import Coq.Logic.FunctionalExtensionality.
+Import ListNotations.
+Require Import Maps.
+Require Import Imp.
+
+
+(** In midterm, we extends the optional [add_for_loop] exercise from
+    the [Imp] chapter, and we were asked to extend the language 
+    of commands with C-style [for] loops. Now I want to prove that 
+    for command and while command are equivalent, that is
+    the command:
+
+      for (c1 ; b ; c2) {
+          c3
+      }
+
+    is equivalent to:
+
+       c1 ;
+       WHILE b DO
+         c3 ;
+         c2
+       END
+   are equivalent
+*)
+
+(** first of all , we will add the definition for for loop *)
+
+Inductive com' : Type :=
+  | CSkip' : com'
+  | CAss' : id -> aexp -> com'
+  | CSeq' : com' -> com' -> com'
+  | CIf' : bexp -> com' -> com' -> com'
+  | CWhile' : bexp -> com' -> com'
+  | CFor' : com' -> bexp -> com' -> com' -> com'.
+
+Inductive ceval' : com' -> state -> state -> Prop :=
+  | E_Skip' : forall st, 
+      ceval' CSkip' st st
+  | E_Ass' : forall st a1 n x, 
+      aeval st a1 = n -> 
+      ceval' (CAss' x a1) st (t_update st x n)
+  | E_Seq' : forall c1 c2 st st' st'', 
+      ceval' c1 st st' -> 
+      ceval' c2 st' st'' -> 
+      ceval' (CSeq' c1 c2) st st''
+  | E_IfTrue' : forall st st' b c1 c2,
+      beval st b = true -> 
+      ceval' c1 st st' -> 
+      ceval' (CIf' b c1 c2) st st'
+  | E_IfFalse' : forall st st' b c1 c2,
+      beval st b = false -> 
+      ceval' c2 st st' -> 
+      ceval' (CIf' b c1 c2) st st'
+  | E_WhileEnd' : forall b st c,
+      beval st b = false ->
+      ceval' (CWhile' b c) st st
+  | E_WhileLoop' : forall st st' st'' b c,
+      beval st b = true ->
+      ceval' c st st' ->
+      ceval' (CWhile' b c) st' st'' ->
+      ceval' (CWhile' b c) st st''
+  | E_For' : forall st st' st'' b c1 c2 c3,
+      ceval' c1 st st' ->
+      ceval' (CWhile' b (CSeq' c2 c3)) st' st'' ->
+      ceval' (CFor' c1 b c2 c3) st st''.
+(** [] *)
+
+Definition cequiv_for_while (c1 c2 : com') : Prop :=
+  forall st st' : state, ceval' c1 st st' <-> ceval' c2 st st'.
+
+Theorem for_while_equiv : forall b c1 c2 c3,
+  cequiv_for_while (CFor' c1 b c2 c3) (CSeq' c1 (CWhile' b (CSeq' c2 c3))).
+Proof.
+  unfold cequiv_for_while.
+  split; intros.
+  - (* -> *)
+    inversion H; subst.
+    apply E_Seq' with st'0.
+    apply H6.
+    apply H7.
+  - (* <- *)
+    inversion H; subst.
+    apply E_For' with st'0.
+    apply H2.
+    apply H5.
+Qed.
+
+
+
+
