final project/NonDeterministic.v
@@ -1,0 +1,512 @@
+(**
+*  CS386L Programming Languages
+* Final project
+* Tian Zhang (tz3272)
+* Brief Introduction:
+*     For the this file, I am working on non-deteminisitic imp, and 
+      all the work is based on Maps, Imp in class. I got some idea from
+      the book, optional exercise from equiv.v
+*)
+
+Require Import ProgramEquivalence.
+Require Import ProgramNotEquivalence.
+Require Import Coq.Bool.Bool.
+Require Import Coq.Arith.Arith.
+Require Import Coq.Arith.EqNat.
+Require Import Coq.omega.Omega.
+Require Import Coq.Lists.List.
+Require Import Coq.Logic.FunctionalExtensionality.
+Import ListNotations.
+Require Import Maps.
+Require Import Imp.
+
+
+(**  Imp's evaluation relation is deterministic.  However,
+    non_determinism is an important part of the definition of many
+    real programming languages. 
+    
+    We will extend Imp with a simple
+    nondeterministic command 
+    
+    The new command has the syntax [HAVOC X],
+    where [X] is an identifier. The effect of executing [HAVOC X] is
+    to assign an arbitrary number to the variable [X],
+    nondeterministically. 
+    
+    For example, after executing the program:
+
+      HAVOC Y;;
+      Z ::= Y * 2
+
+    the value of [Y] can be any number, while the value of [Z] is
+    twice that of [Y] (so [Z] is always even). 
+    
+    In other word, a variable on which we do [HAVOC] roughly corresponds
+    to an unitialized variable in a low-level language like C.  After
+    the [HAVOC], the variable holds a fixed but arbitrary number.  Most
+    sources of nondeterminism in language definitions are there
+    precisely because programmers don't care which choice is made 
+*)
+
+
+(** To formalize this new imp, we first add a clause to the definition of
+    commands. *)
+
+Inductive com : Type :=
+  | CSkip : com
+  | CAss : id -> aexp -> com
+  | CSeq : com -> com -> com
+  | CIf : bexp -> com -> com -> com
+  | CWhile : bexp -> com -> com
+  | CHavoc : id -> com.                (* new *)
+
+Notation "'SKIP'" :=
+  CSkip.
+Notation "X '::=' a" :=
+  (CAss X a) (at level 60).
+Notation "c1 ;; c2" :=
+  (CSeq c1 c2) (at level 80, right associativity).
+Notation "'WHILE' b 'DO' c 'END'" :=
+  (CWhile b c) (at level 80, right associativity).
+Notation "'IFB' e1 'THEN' e2 'ELSE' e3 'FI'" :=
+  (CIf e1 e2 e3) (at level 80, right associativity).
+Notation "'HAVOC' l" := (CHavoc l) (at level 60).
+
+
+(** Now, we must extend the operational semantics. define ceval for this
+  new HAVOC
+*)
+
+Reserved Notation "c1 '/' st '\\' st'"
+                  (at level 40, st at level 39).
+
+Inductive ceval : com -> state -> state -> Prop :=
+  | E_Skip : forall st : state, SKIP / st \\ st
+  | E_Ass : forall (st : state) (a1 : aexp) (n : nat) (X : id),
+      aeval st a1 = n ->
+      (X ::= a1) / st \\ t_update st X n
+  | E_Seq : forall (c1 c2 : com) (st st' st'' : state),
+      c1 / st \\ st' ->
+      c2 / st' \\ st'' ->
+      (c1 ;; c2) / st \\ st''
+  | E_IfTrue : forall (st st' : state) (b1 : bexp) (c1 c2 : com),
+      beval st b1 = true ->
+      c1 / st \\ st' ->
+      (IFB b1 THEN c1 ELSE c2 FI) / st \\ st'
+  | E_IfFalse : forall (st st' : state) (b1 : bexp) (c1 c2 : com),
+      beval st b1 = false ->
+      c2 / st \\ st' ->
+      (IFB b1 THEN c1 ELSE c2 FI) / st \\ st'
+  | E_WhileEnd : forall (b1 : bexp) (st : state) (c1 : com),
+      beval st b1 = false -> 
+      (WHILE b1 DO c1 END) / st \\ st
+  | E_WhileLoop : forall (st st' st'' : state) (b1 : bexp) (c1 : com),
+      beval st b1 = true ->
+      c1 / st \\ st' ->
+      (WHILE b1 DO c1 END) / st' \\ st'' ->
+      (WHILE b1 DO c1 END) / st \\ st''
+  | E_Havoc : forall (st : state) (i : id) (n : nat),
+      (HAVOC i) / st \\ (t_update st i n)
+
+  where "c1 '/' st '\\' st'" := (ceval c1 st st').
+
+
+(** next, we repeat the definition of command equivalence from above: *)
+
+Definition cequiv (c1 c2 : com) : Prop := forall st st' : state,
+  c1 / st \\ st' <-> c2 / st \\ st'.
+
+(** The next step is to prove some nondeterministic
+    programs equivalent / inequivalent. *)
+
+
+Definition pXY :=
+  HAVOC X;; HAVOC Y.
+
+Definition pYX :=
+  HAVOC Y;; HAVOC X.
+
+
+
+Theorem pXY_cequiv_pYX :
+  cequiv pXY pYX \/ ~cequiv pXY pYX.
+Proof.
+left.
+  unfold cequiv.
+  split; intros;
+    inversion H; subst;
+    inversion H2; subst;
+    inversion H5; subst.
+  -(* -> *)
+    replace (t_update (t_update st X n) Y n0) with (t_update (t_update st Y n0) X n).
+    apply E_Seq with (t_update st Y n0).
+    apply E_Havoc.
+    apply E_Havoc.
+    apply functional_extensionality; intros.
+    rewrite t_update_permute. reflexivity.
+    unfold not.
+    intros.
+    inversion H0.
+  - (* <- *)
+    replace (t_update (t_update st Y n) X n0) with (t_update (t_update st X n0) Y n).
+    apply E_Seq with (t_update st X n0).
+    apply E_Havoc.
+    apply E_Havoc.
+    apply functional_extensionality; intros.
+    rewrite t_update_permute. reflexivity.
+    unfold not.
+    intros.
+    inversion H0.
+Qed.
+
+
+(** Here is the second example, havoc_copy *)
+
+
+Definition ptwice :=
+  HAVOC X;; HAVOC Y.
+
+Definition pcopy :=
+  HAVOC X;; Y ::= AId X.
+
+Theorem ptwice_cequiv_pcopy :
+  cequiv ptwice pcopy \/ ~cequiv ptwice pcopy.
+Proof.
+  right.
+  unfold not.
+  intros contra.
+  unfold cequiv in contra.
+  assert (ptwice / empty_state \\ t_update (t_update empty_state X 1) Y 2) as PT.
+  apply E_Seq with (st':=t_update empty_state X 1).
+  apply E_Havoc.
+  apply E_Havoc.
+  assert (pcopy / empty_state \\ t_update (t_update empty_state X 1) Y 2) as PC.
+  apply contra; assumption.
+  inversion PC; inversion PT; subst.
+  inversion H1; inversion H7; subst.
+  inversion H10; inversion H4; subst.
+  unfold t_update at 3 in H9.
+  simpl in H9.
+  remember (beq_nat n 1).
+  destruct b.
+  - (* n = 1 *)
+    apply beq_nat_eq in Heqb.
+    rewrite Heqb in *.
+    inversion H9.
+    assert (t_update (t_update empty_state X 1) Y 1 Y = t_update (t_update empty_state X 1) Y 2 Y).
+    rewrite H2. reflexivity.
+    rewrite t_update_eq in H0.
+    symmetry in H0.
+    rewrite t_update_eq in H0.
+    inversion H0.
+  - (* n != 1 *)
+    assert (t_update (t_update empty_state X n) Y n X = t_update (t_update empty_state X 1) Y 2 X).
+    rewrite H9. reflexivity.
+    unfold t_update in H0. simpl in H0. rewrite H0 in Heqb. inversion Heqb.
+Qed.
+
+(** This part illustrate the phenomenon of nondeterministic about loop.
+    In a language,
+    with nondeterminism, some programs always terminate,
+    some programs always diverge, and some programs can
+    nondeterministically terminate in some runs and diverge in
+    others. 
+*)
+
+(** below part is the advanced exercise in equiv.v about nondeterminism  *)
+
+(** Prove that [p1] and [p2] are equivalent. *)
+
+
+Definition p1 : com :=
+  WHILE (BNot (BEq (AId X) (ANum 0))) DO
+    HAVOC Y;;
+    X ::= APlus (AId X) (ANum 1)
+  END.
+
+Definition p2 : com :=
+  WHILE (BNot (BEq (AId X) (ANum 0))) DO
+    SKIP
+  END.
+
+(** Intuitively, the programs have the same termination
+    behavior: either they loop forever, or they terminate in the
+    same state they started in.  
+    
+    We can capture the termination
+    behavior of [p1] and [p2] individually with these lemmas: *)
+
+Lemma WHILE_true_nonterm : forall (P : state -> Prop) (b : bexp) (c : com),
+  (forall (st : state), P st -> beval st b = true) ->
+  (forall (st st' : state), P st -> c / st \\ st' -> P st') ->
+  (forall (st st' : state), P st -> ~((WHILE b DO c END) / st \\ st')).
+Proof.
+  intro P.
+  intros b c.
+  intros Hb Hc.
+  intros st st'.
+  intro HP.
+  intro Contra.
+  remember (WHILE b DO c END) as cw.
+  induction Contra;
+  (* Trivial, contradiction cases. *)
+  try (inversion Heqcw);
+  subst.
+  (* E_WhileEnd *)
+  rewrite -> Hb in H.
+  inversion H.
+  assumption.
+  (* E_WhileLoop *)
+  apply IHContra2.
+  eapply Hc.
+  apply HP.
+  apply Contra1.
+  reflexivity. Qed.
+
+
+Lemma p1p2_cond_eval : forall (st : state),
+  st X <> 0 ->
+  beval st (BNot (BEq (AId X) (ANum 0))) = true.
+Proof.
+  intro st.
+  intro H.
+  simpl.
+  apply negb_true_iff.
+  apply beq_nat_false_iff.
+  assumption. Qed.
+  
+
+Lemma p1_may_diverge : forall st st', st X <> 0 ->
+  ~ p1 / st \\ st'.
+Proof. 
+  intros st st'.
+  intro HX.
+  apply WHILE_true_nonterm with (P := fun st => st X <> 0).
+
+  apply p1p2_cond_eval.
+
+  intros st0 st'0.
+  intros HP Hc.
+  inversion Hc. subst.
+  inversion H1. subst.
+  inversion H4. subst.
+  unfold update.
+  simpl.
+  apply not_eq_sym.
+  rewrite <- plus_comm.
+  apply O_S.
+
+  assumption. Qed.
+
+Lemma p2_may_diverge : forall st st', st X <> 0 ->
+  ~ p2 / st \\ st'.
+Proof.
+  intros st st'.
+  intro HX.
+  apply WHILE_true_nonterm with (P := fun st => st X <> 0).
+
+  apply p1p2_cond_eval.
+
+  intros st0 st'0.
+  intros HP Hc.
+  inversion Hc. subst.
+  apply HP.
+
+  assumption. Qed.
+
+(** Next, use those lemmas to prove that [p1] and [p2] are actually
+    equivalent. *)
+
+Theorem p1_p2_equiv : cequiv p1 p2.
+Proof.
+  unfold cequiv.
+  intros st st'.
+  destruct (eq_nat_dec (st X) 0).
+
+  (* st X = 0 *)
+  split;
+  intro H;
+  inversion H; subst;
+  try (apply E_WhileEnd;
+       simpl;
+       rewrite -> e;
+       reflexivity);
+  try (simpl in H2;
+       rewrite -> e in H2;
+       simpl in H2;
+       inversion H2).
+
+  (* st X <> 0 *)
+  split;
+  intro H;
+  try (apply p1_may_diverge in H);
+  try (apply p2_may_diverge in H);
+  try (contradiction H);
+  assumption. 
+Qed.
+
+
+(** Below is part of advanced exercise in equiv.v about nondeterminism
+    Prove that the following programs are not equivalent. 
+*)
+
+Definition p3 : com :=
+  Z ::= ANum 1;;
+  WHILE (BNot (BEq (AId X) (ANum 0))) DO
+    HAVOC X;;
+    HAVOC Z
+  END.
+
+Definition p4 : com :=
+  X ::= (ANum 0);;
+  Z ::= (ANum 1).
+
+
+Definition st_X1 : state := t_update empty_state X 1.
+Definition st_Z0_X0 : state := t_update (t_update st_X1 Z 0) X 0.
+
+Lemma p3_X0_Z0 :
+  p3 / st_X1 \\ st_Z0_X0.
+Proof.
+  unfold p3.
+  eapply E_Seq.
+  apply E_Ass.
+  reflexivity.
+  apply E_WhileLoop with (st' := t_update (t_update (t_update st_X1 Z 1) X 0) Z 0).
+  reflexivity.
+  apply E_Seq with (st' := t_update (t_update st_X1 Z 1) X 0).
+  apply E_Havoc.
+  apply E_Havoc.
+  assert (eval : t_update (t_update (t_update st_X1 Z 1) X 0) Z 0
+               = t_update (t_update st_X1 Z 0) X 0).
+    unfold t_update.
+    apply functional_extensionality.
+    intro V.
+    destruct (beq_id Z V);
+    destruct (beq_id X V);
+    reflexivity.
+  rewrite -> eval.
+  apply E_WhileEnd.
+  reflexivity. Qed.
+
+Theorem p3_p4_inequiv : ~ cequiv p3 p4.
+Proof.
+  unfold cequiv.
+  intro Contra.
+  assert (H : p3 / st_X1 \\ st_Z0_X0).
+    apply p3_X0_Z0.
+
+  apply Contra in H.
+  unfold p4 in H.
+  inversion H. subst.
+  inversion H2. subst.
+  inversion H5. subst.
+  simpl in H6.
+
+  assert (H0 : st_Z0_X0 Z = 0).
+    reflexivity.
+  assert (H1 : st_Z0_X0 Z = 1).
+    rewrite <- H6.
+    reflexivity.
+  rewrite -> H0 in H1.
+  inversion H1. Qed.
+ 
+ 
+(** below example is  5 stars advanced exercise in equiv.v 
+  proof that program p5 and p6 are equivalent
+*)
+
+Definition p5 : com :=
+  WHILE (BNot (BEq (AId X) (ANum 1))) DO
+    HAVOC X
+  END.
+
+Definition p6 : com :=
+  X ::= ANum 1.
+
+(** to prove the equivalence of these 2 program, cequiv is hard to achieve
+at once.
+    As a result, I introduce clequiv, that simple has the left side of cequiv
+    So, I will prove clequiv p5 p6 and then clequiv p6 p5.
+    Finally, prove that cequiv p5 p6.
+
+*)
+Definition clequiv (c1 c2 : com) := forall (st st' : state),
+  c1 / st \\ st' -> c2 / st \\ st'.
+  
+Lemma p5_p6_lequiv : clequiv p5 p6.
+Proof.
+  intros st st'.
+  intro H.
+  remember p5 as p5c.
+  unfold p6.
+  induction H;
+  (* Trivial, contradiction cases. *)
+  try (inversion Heqp5c);
+  subst.
+  (* E_WhileEnd *)
+  simpl in H.
+  rewrite -> negb_false_iff in H.
+  apply beq_nat_true_iff in H.
+  assert (Hst : t_update st X 1 = st).
+    apply functional_extensionality.
+    intro V. rewrite <- H.
+    rewrite-> t_update_same. reflexivity.
+  rewrite <- Hst at 2.
+  apply E_Ass.
+  reflexivity.
+  (* E_WhileLoop *)
+  assert (Hass : p6 / st' \\ st'').
+    apply IHceval2.
+    assumption.
+  clear IHceval1 IHceval2 Heqp5c H H1.
+  inversion H0. subst.
+  inversion Hass. subst.
+  assert (Hsimpl : t_update (t_update st X n) X (aeval (t_update st X n) (ANum 1))
+           = t_update st X 1).
+    simpl.
+    apply functional_extensionality.
+    intro V.
+    rewrite -> t_update_shadow. reflexivity.
+  rewrite -> Hsimpl.
+  apply E_Ass.
+  reflexivity. Qed.
+  
+Lemma p6_p5_lequiv : clequiv p6 p5.
+Proof.
+  unfold p6.
+  unfold p5.
+  intros st st'.
+  intro H.
+  inversion H; subst.
+  destruct (eq_nat_dec (st X) 1).
+  (* X = 1 *)
+  assert (Hsimpl : t_update st X (aeval st (ANum 1)) = st).
+    apply functional_extensionality.
+    intro V. simpl. rewrite <- e.
+    rewrite -> t_update_same.
+    reflexivity.
+  rewrite -> Hsimpl.
+  apply E_WhileEnd.
+  simpl.
+  rewrite -> e.
+  reflexivity.
+  (* X <> 1 *)
+  eapply E_WhileLoop.
+  simpl.
+  rewrite -> negb_true_iff.
+  apply beq_nat_false_iff.
+  assumption.
+  unfold beq_nat.
+  apply E_Havoc.
+  apply E_WhileEnd.
+  reflexivity. Qed.
+
+Theorem p5_p6_equiv : cequiv p5 p6.
+Proof. 
+  split.
+  apply p5_p6_lequiv.
+  apply p6_p5_lequiv. 
+Qed.
+
+
