final project/ProgramEquivalence.v
@@ -1,0 +1,593 @@
+(**
+*  CS386L Programming Languages
+* Final project
+* Tian Zhang (tz3272)
+* Brief Introduction:
+*     This file contains proof for program equivalence, a starting point
+*     For my final project
+*     All the proof is based on Imp.v 
+*     Some example and proof are followed content from equiv.v
+*)
+
+Require Import Coq.Bool.Bool.
+Require Import Coq.Arith.Arith.
+Require Import Coq.Arith.EqNat.
+Require Import Coq.omega.Omega.
+Require Import Coq.Lists.List.
+Require Import Coq.Logic.FunctionalExtensionality.
+Import ListNotations.
+Require Import Maps.
+Require Import Imp.
+
+
+(** Two aexp or bexp are behaviorally equivalent if they
+    evaluate to the same result in every state *)
+
+Definition aequiv (a1 a2 : aexp) : Prop :=
+  forall (st:state),
+    aeval st a1 = aeval st a2.
+
+Definition bequiv (b1 b2 : bexp) : Prop :=
+  forall (st:state),
+    beval st b1 = beval st b2.
+
+(** Two commands are behaviorally equivalent
+    if, for any given starting state, they either both diverge or both
+    terminate in the same final state.*)
+
+Definition cequiv (c1 c2 : com) : Prop :=
+  forall (st st' : state),
+    (c1 / st \\ st') <-> (c2 / st \\ st').
+
+
+(** Here is some command equivalent example*)
+
+(** SKIP , skip in command left and skip in command right*)
+
+Theorem skip_left: forall c,
+  cequiv 
+     (SKIP;; c) 
+     c.
+Proof. 
+  intros c st st'.
+  split; intros H.
+  - (* -> *) 
+    inversion H. subst. 
+    inversion H2. subst. 
+    assumption.
+  - (* <- *) 
+    apply E_Seq with st.
+    apply E_Skip. 
+    assumption.  
+Qed.
+
+
+Theorem skip_right: forall c,
+  cequiv 
+    (c;; SKIP) 
+    c.
+Proof.
+  intros.
+  split; intros.
+  - (* -> *)
+    inversion H.
+    simpl. subst. inversion H5.
+    subst.
+    assumption.
+  - (* <- *)
+  apply E_Seq with st'.
+  assumption.
+  apply E_Skip.
+Qed.
+
+(** IFB, (IFB b THEN c1 ELSE c2 FI), if clause evaluate to true , 
+    then goto c1
+    If evaluate to false, then goto c2
+*)
+
+
+Theorem IFB_true: forall b c1 c2,
+     bequiv b BTrue  ->
+     cequiv
+       (IFB b THEN c1 ELSE c2 FI)
+       c1.
+Proof.
+  intros b c1 c2 Hb.
+  split; intros H.
+  - (* -> *)
+    inversion H; subst.
+    + (* b == true *)
+      assumption.
+    + (* b == false *)
+      unfold bequiv in Hb. simpl in Hb.
+      rewrite Hb in H5.
+      inversion H5.
+  - (* <- *)
+    apply E_IfTrue; try assumption.
+    unfold bequiv in Hb. simpl in Hb.
+    rewrite Hb. reflexivity.  Qed.
+
+
+Theorem IFB_false: forall b c1 c2,
+  bequiv b BFalse  ->
+  cequiv
+    (IFB b THEN c1 ELSE c2 FI)
+    c2.
+Proof.
+  intros b c1 c2 Hb.
+  split; intros H.
+  - (* -> *)
+    inversion H; subst.
+    + (* b => true *)
+    unfold bequiv in Hb.
+    rewrite Hb in H5. inversion H5.
+    + (* b => false *)
+    assumption.
+  - (* <- *)
+    apply E_IfFalse.
+    unfold bequiv in Hb.
+    simpl in Hb. apply Hb.
+    assumption.
+Qed.
+
+
+(** swap_if_branches,
+    swap the if else cases by negating the if clause
+  *)
+
+Lemma beval_neg : forall st b b',
+                    beval st (BNot b) = b' -> beval st b = negb b'.
+Proof.
+  intros.
+  destruct b'; simpl in H; symmetry in H; apply negb_sym in H; assumption.
+Qed. 
+
+Theorem swap_if_branches: forall b e1 e2,
+  cequiv
+    (IFB b THEN e1 ELSE e2 FI)
+    (IFB BNot b THEN e2 ELSE e1 FI).
+Proof.
+  intros.
+  split; intros.
+  - (* -> *)
+  inversion H; subst.
+  apply E_IfFalse. simpl. rewrite H5. reflexivity.
+  assumption.
+  apply E_IfTrue. simpl. rewrite H5. reflexivity.
+  assumption.
+  - (* <- *)
+  inversion H; subst.
+    + (* False *)
+    apply E_IfFalse.
+    apply beval_neg in H5; simpl in H5; assumption.
+    assumption.
+    + (*True *)
+    apply E_IfTrue.
+    apply beval_neg in H5; simpl in H5; assumption.
+    assumption.
+Qed.
+
+
+(** WHILE loops, if while clause evaluate to false, then it is similar
+  to skip
+ *)
+
+Theorem WHILE_false : forall b c,
+     bequiv b BFalse ->
+     cequiv
+       (WHILE b DO c END)
+       SKIP.
+Proof.
+  intros b c Hb. split; intros H.
+  - (* -> *)
+    inversion H; subst.
+    + (* E_WhileEnd *)
+      apply E_Skip.
+    + (* E_WhileLoop *)
+      rewrite Hb in H2. inversion H2.
+  - (* <- *)
+    inversion H; subst.
+    apply E_WhileEnd.
+    rewrite Hb.
+    reflexivity.  Qed.
+
+
+
+(** When while clause evaluate to true, it will never terminate,
+    Here is the lemma,
+
+    If b is equivalent to [BTrue], then it cannot be the
+    case that [(WHILE b DO c END) / st \\ st'].
+*)
+
+Lemma WHILE_true_nonterm : forall b c st st',
+     bequiv b BTrue ->
+     ~( (WHILE b DO c END) / st \\ st' ).
+Proof.
+
+  intros b c st st' Hb.
+  intros H.
+  remember (WHILE b DO c END) as cw eqn:Heqcw.
+  induction H;
+    (*by inversion *)
+    inversion Heqcw; subst; clear Heqcw.
+  - (* E_WhileEnd *) (* contradictory -- b is always true! *)
+    unfold bequiv in Hb.
+    (* [rewrite] is able to instantiate the quantifier in [st] *)
+    rewrite Hb in H. inversion H.
+  - (* E_WhileLoop *) (* immediate from the IH *)
+    apply IHceval2. reflexivity.  Qed.
+
+
+(** now we have lemma, we can evaluate while true *)
+
+Theorem ex_falso_quodlibet : forall (P:Prop), False -> P.
+Proof.
+  intros. inversion H.
+Qed.
+
+Lemma skip_state : forall st st',
+                     SKIP / st \\ st' -> st = st'.
+Proof.
+  intros.
+  inversion H. subst.
+  reflexivity.
+Qed.
+
+
+Theorem WHILE_true: forall b c,
+     bequiv b BTrue  ->
+     cequiv
+       (WHILE b DO c END)
+       (WHILE BTrue DO SKIP END).
+Proof.
+  intros.
+  intros st st'. split.
+  - (* -> *) 
+    intros.
+    apply WHILE_true_nonterm with (c:=c) (st:=st) (st':=st') in H.
+    apply ex_falso_quodlibet.
+    apply H in H0. assumption.
+  - (* <- *)
+  intros.
+  remember (WHILE BTrue DO SKIP END).
+  induction H0; inversion Heqc0. 
+    + (* E_WhileEnd *)
+  subst. simpl in H0. inversion H0.
+    + (* E_WhileLoop *)
+  subst.
+  clear IHceval1.
+  rename H0_ into Hst.
+  apply skip_state in Hst.
+  rewrite Hst.
+  apply IHceval2.
+  assumption.
+Qed.
+
+
+(** another key concept in loop is loop unrolling , programms are
+    behaviorally equivalent if we perform the loop unrolling
+*)
+
+Theorem loop_unrolling: forall b c,
+  cequiv
+    (WHILE b DO c END)
+    (IFB b THEN (c;; WHILE b DO c END) ELSE SKIP FI).
+Proof.
+  intros b c st st'.
+  split; intros Hce.
+  - (* -> *)
+    inversion Hce; subst.
+    + (* loop doesn't run *)
+      apply E_IfFalse. assumption. apply E_Skip.
+    + (* loop runs *)
+      apply E_IfTrue. assumption.
+      apply E_Seq with (st' := st'0). assumption. assumption.
+  - (* <- *)
+    inversion Hce; subst.
+    + (* loop runs *)
+      inversion H5; subst.
+      apply E_WhileLoop with (st' := st'0).
+      assumption. assumption. assumption.
+    + (* loop doesn't run *)
+      inversion H5; subst. apply E_WhileEnd. assumption.  Qed.
+
+
+(** change the associativity of command *)
+
+
+Theorem seq_assoc : forall c1 c2 c3,
+  cequiv ((c1;;c2);;c3) (c1;;(c2;;c3)).
+Proof.
+ intros.
+  split; intros.
+  - (* -> *)
+  inversion H; subst.
+  inversion H2; subst.
+  apply E_Seq with (st':=st'1).
+  assumption.
+  apply E_Seq with (st':=st'0).
+  assumption.
+  assumption.
+  - (* <- *)
+  inversion H; subst.
+  inversion H5; subst.
+  apply E_Seq with (st':=st'1).
+  apply E_Seq with (st':=st'0).
+  assumption.
+  assumption.
+  assumption.
+Qed.
+
+
+(** Assignment , simple example is like indentity assignment *)
+
+Theorem identity_assignment : forall (X:id),
+  cequiv
+    (X ::= AId X)
+    SKIP.
+Proof.
+   intros. split; intro H.
+     - (* -> *)
+       inversion H; subst. simpl.
+       replace (t_update st X (st X)) with st.
+       + constructor.
+       + apply functional_extensionality. intro.
+         rewrite t_update_same; reflexivity.
+     - (* <- *)
+       replace st' with (t_update st' X (aeval st' (AId X))).
+       + inversion H. subst. apply E_Ass. reflexivity.
+       + apply functional_extensionality. intro.
+         rewrite t_update_same. reflexivity.
+Qed.
+
+(** Another theorem about assignment simple, no need to assign twices
+if X already evaluate to e*)
+
+
+Theorem assign_aequiv : forall X e,
+  aequiv (AId X) e ->
+  cequiv SKIP (X ::= e).
+Proof.
+intros.
+  split; intro He.
+  - (* -> *)
+  apply skip_state in He.
+  unfold aequiv in H.
+  assert (st' = (t_update st' X (st' X))).
+    apply functional_extensionality. intro.
+    rewrite t_update_same; reflexivity.
+  rewrite H0.
+  rewrite He.
+  apply E_Ass.
+  rewrite <- H.
+  simpl. reflexivity.
+  - (* <- *)
+  inversion He.
+  subst.
+  assert (st = t_update st X (st X)).
+    apply functional_extensionality. intros.
+    rewrite t_update_same; reflexivity.
+  rewrite H0 in He at 1.
+  inversion He.
+  rewrite <- H0 in H4.
+  unfold aequiv in H.
+  rewrite <- H in H5.
+  simpl in H5.
+  rewrite H5.
+  rewrite <- H0.
+  apply E_Skip.
+Qed.
+
+
+
+
+
+(** Now we show the detail of program equivalence, and the next step
+is show the  Properties of Behavioral Equivalence , in order to help further
+proof about constant folding and partial evaluation
+*)
+
+(** First, we verify that the equivalences on aexps, bexps, and
+    coms are eflexive,
+    symmetric, and transitive. *)
+
+Lemma refl_aequiv : forall (a : aexp), aequiv a a.
+Proof.
+  intros a st. reflexivity.  Qed.
+
+Lemma sym_aequiv : forall (a1 a2 : aexp),
+  aequiv a1 a2 -> aequiv a2 a1.
+Proof.
+  intros a1 a2 H. intros st. symmetry. apply H.  Qed.
+
+Lemma trans_aequiv : forall (a1 a2 a3 : aexp),
+  aequiv a1 a2 -> aequiv a2 a3 -> aequiv a1 a3.
+Proof.
+  unfold aequiv. intros a1 a2 a3 H12 H23 st.
+  rewrite (H12 st). rewrite (H23 st). reflexivity.  Qed.
+
+Lemma refl_bequiv : forall (b : bexp), bequiv b b.
+Proof.
+  unfold bequiv. intros b st. reflexivity.  Qed.
+
+Lemma sym_bequiv : forall (b1 b2 : bexp),
+  bequiv b1 b2 -> bequiv b2 b1.
+Proof.
+  unfold bequiv. intros b1 b2 H. intros st. symmetry. apply H.  Qed.
+
+Lemma trans_bequiv : forall (b1 b2 b3 : bexp),
+  bequiv b1 b2 -> bequiv b2 b3 -> bequiv b1 b3.
+Proof.
+  unfold bequiv. intros b1 b2 b3 H12 H23 st.
+  rewrite (H12 st). rewrite (H23 st). reflexivity.  Qed.
+
+Lemma refl_cequiv : forall (c : com), cequiv c c.
+Proof.
+  unfold cequiv. intros c st st'. apply iff_refl.  Qed.
+
+Lemma sym_cequiv : forall (c1 c2 : com),
+  cequiv c1 c2 -> cequiv c2 c1.
+Proof.
+  unfold cequiv. intros c1 c2 H st st'.
+  assert (c1 / st \\ st' <-> c2 / st \\ st') as H'.
+  { (* Proof of assertion *) apply H. }
+  apply iff_sym. assumption.
+Qed.
+
+Lemma iff_trans : forall (P1 P2 P3 : Prop),
+  (P1 <-> P2) -> (P2 <-> P3) -> (P1 <-> P3).
+Proof.
+  intros P1 P2 P3 H12 H23.
+  inversion H12. inversion H23.
+  split; intros A.
+    apply H1. apply H. apply A.
+    apply H0. apply H2. apply A.  Qed.
+
+Lemma trans_cequiv : forall (c1 c2 c3 : com),
+  cequiv c1 c2 -> cequiv c2 c3 -> cequiv c1 c3.
+Proof.
+  unfold cequiv. intros c1 c2 c3 H12 H23 st st'.
+  apply iff_trans with (c2 / st \\ st'). apply H12. apply H23.  Qed.
+
+
+(** The next step is to prove Behavioral Equivalence is a Congruence 
+    That is, the equivalence of two subprograms implies the
+    equivalence of the larger programs in which they are embedded:
+
+
+              cequiv c1 c1'
+              cequiv c2 c2'
+         ------------------------
+         cequiv (c1;;c2) (c1';;c2')
+*)
+
+
+(** First, aquiv cases, which is simple,
+              aequiv a1 a1'
+      -----------------------------
+      cequiv (i ::= a1) (i ::= a1')
+*)
+
+Theorem CAss_congruence : forall i a1 a1',
+  aequiv a1 a1' ->
+  cequiv (CAss i a1) (CAss i a1').
+Proof.
+  intros i a1 a2 Heqv st st'.
+  split; intros Hceval.
+  - (* -> *)
+    inversion Hceval. subst. apply E_Ass.
+    rewrite Heqv. reflexivity.
+  - (* <- *)
+    inversion Hceval. subst. apply E_Ass.
+    rewrite Heqv. reflexivity.  Qed.
+    
+(** Next case is while loop,
+                    bequiv b1 b1'
+      --------------------------------------------------
+      cequiv (WHILE b1 DO c1 END) (WHILE b1' DO c1' END).
+*)
+Theorem CWhile_congruence : forall b1 b1' c1 c1',
+  bequiv b1 b1' -> cequiv c1 c1' ->
+  cequiv (WHILE b1 DO c1 END) (WHILE b1' DO c1' END).
+Proof.
+  unfold bequiv,cequiv.
+  intros b1 b1' c1 c1' Hb1e Hc1e st st'.
+  split; intros Hce.
+  - (* -> *)
+    remember (WHILE b1 DO c1 END) as cwhile
+      eqn:Heqcwhile.
+    induction Hce; inversion Heqcwhile; subst.
+    + (* E_WhileEnd *)
+      apply E_WhileEnd. rewrite <- Hb1e. apply H.
+    + (* E_WhileLoop *)
+      apply E_WhileLoop with (st' := st').
+      * (* show loop runs *) rewrite <- Hb1e. apply H.
+      * (* body execution *)
+        apply (Hc1e st st').  apply Hce1.
+      * (* subsequent loop execution *)
+        apply IHHce2. reflexivity.
+  - (* <- *)
+    remember (WHILE b1' DO c1' END) as c'while
+      eqn:Heqc'while.
+    induction Hce; inversion Heqc'while; subst.
+    + (* E_WhileEnd *)
+      apply E_WhileEnd. rewrite -> Hb1e. apply H.
+    + (* E_WhileLoop *)
+      apply E_WhileLoop with (st' := st').
+      * (* show loop runs *) rewrite -> Hb1e. apply H.
+      * (* body execution *)
+        apply (Hc1e st st').  apply Hce1.
+      * (* subsequent loop execution *)
+        apply IHHce2. reflexivity.  Qed.
+
+(** the next case is about command sequence
+                    cequiv c1 c1' 
+                    cequiv c2 c2'
+           -----------------------------
+           cequiv (c1;;c2) (c1';;c2').
+*)
+Theorem CSeq_congruence : forall c1 c1' c2 c2',
+  cequiv c1 c1' -> cequiv c2 c2' ->
+  cequiv (c1;;c2) (c1';;c2').
+Proof.
+  intros. unfold cequiv. split; intros He.
+  - (* <- *)
+  unfold cequiv in *. inversion He. subst.
+  apply H with (st':=st'0) in H3.
+  apply H0 with (st:=st'0) in H6.
+  apply E_Seq with (st':=st'0). assumption.
+  assumption.
+  - (* -> *)
+  unfold cequiv in *.
+  inversion He. subst.
+  apply H with (st':=st'0) in H3.
+  apply H0 with (st:=st'0) in H6.
+  apply E_Seq with (st':=st'0).
+  assumption.
+  assumption.
+Qed.
+
+(** The final case is about if
+                    bequiv b b'
+                    cequiv c1 c1' 
+                    cequiv c2 c2'
+         ----------------------------------------------------
+   cequiv (IFB b THEN c1 ELSE c2 FI) (IFB b' THEN c1' ELSE c2' FI).
+
+*)
+Theorem CIf_congruence : forall b b' c1 c1' c2 c2',
+  bequiv b b' -> cequiv c1 c1' -> cequiv c2 c2' ->
+  cequiv (IFB b THEN c1 ELSE c2 FI)
+         (IFB b' THEN c1' ELSE c2' FI).
+Proof.
+  intros.
+  unfold cequiv.
+  split; intro He.
+  - (* -> *)
+  unfold cequiv in *.
+  unfold bequiv in H.
+  inversion He; subst.
+    + (* b => true *)
+    apply E_IfTrue. rewrite H in H7. assumption.
+    rewrite H0 in H8. assumption.
+    + (* b => false *)
+    apply E_IfFalse. rewrite H in H7. assumption.
+    rewrite H1 in H8. assumption.
+  - (* <- *)
+  unfold cequiv in *.
+  unfold bequiv in H.
+  symmetry in H.
+  inversion He; subst.
+     + (* b => true *)
+  apply E_IfTrue. rewrite H in H7. assumption.
+  rewrite <- H0 in H8. assumption.
+     + (* b => false *)
+  apply E_IfFalse. rewrite H in H7. assumption.
+  rewrite <- H1 in H8. assumption.
+Qed.
+
+(** Now we finish the definition and proof about behaviorally equivalence
+    the next step is to use those definition and proof in constant propagation
+    and partial evaluation
+*)
