final project/ProgramNotEquivalence.v
@@ -1,0 +1,243 @@
+(**
+*  CS386L Programming Languages
+* Final project
+* Tian Zhang (tz3272)
+* Brief Introduction:
+*     For the this file, I am working on program inequivalence, and 
+      all the work is based on Maps, Imp in class. I got some idea from
+      the book
+*)
+
+Require Import ProgramEquivalence.
+Require Import Coq.Bool.Bool.
+Require Import Coq.Arith.Arith.
+Require Import Coq.Arith.EqNat.
+Require Import Coq.omega.Omega.
+Require Import Coq.Lists.List.
+Require Import Coq.Logic.FunctionalExtensionality.
+Import ListNotations.
+Require Import Maps.
+Require Import Imp.
+
+
+(** Now we have prove that program are equivalent,
+ the next step is to prove that programs are not equivalent 
+*)
+
+
+(** First, define a function that substitutes an arithmetic
+    expression for each occurrence of a given variable in another
+    expression: 
+
+       c1  =  (X ::= 4 + 5;; 
+               Y ::= Y + X)
+       c2  =  (X ::= 4 + 5;; 
+               Y ::= Y + (4 + 5))
+    *)
+
+Fixpoint subst_aexp (i : id) (u : aexp) (a : aexp) : aexp :=
+  match a with
+  | ANum n       =>
+      ANum n
+  | AId i'       =>
+      if beq_id i i' then u else AId i'
+  | APlus a1 a2  =>
+      APlus (subst_aexp i u a1) (subst_aexp i u a2)
+  | AMinus a1 a2 =>
+      AMinus (subst_aexp i u a1) (subst_aexp i u a2)
+  | AMult a1 a2  =>
+      AMult (subst_aexp i u a1) (subst_aexp i u a2)
+  end.
+
+Example subst_aexp_ex :
+  subst_aexp X (APlus (ANum 42) (ANum 53))
+             (APlus (AId Y) (AId X)) 
+= (APlus (AId Y) (APlus (ANum 42) (ANum 53))).
+Proof. reflexivity.  Qed.
+
+(** Now we need to prove that such subsitution are behaviour equivalence
+ *)
+
+Definition subst_equiv_property := forall i1 i2 a1 a2,
+  cequiv (i1 ::= a1;; i2 ::= a2)
+         (i1 ::= a1;; i2 ::= subst_aexp i1 a1 a2).
+
+(** the property does not always hold. Here is the counter example
+
+
+    Consider the following program:
+
+         X ::= APlus (AId X) (ANum 1);; Y ::= AId X
+
+    Note that
+
+         (X ::= APlus (AId X) (ANum 1);; Y ::= AId X)
+         / empty_state \\ st1,
+
+    where [st1 = { X |-> 1, Y |-> 1 }].
+
+    By our assumption, we know that
+
+        cequiv (X ::= APlus (AId X) (ANum 1);; Y ::= AId X)
+               (X ::= APlus (AId X) (ANum 1);; Y ::= APlus (AId X) (ANum 1))
+
+    so, by the definition of [cequiv], we have
+
+        (X ::= APlus (AId X) (ANum 1);; Y ::= APlus (AId X) (ANum 1))
+        / empty_state \\ st1.
+
+    But we can also derive
+
+        (X ::= APlus (AId X) (ANum 1);; Y ::= APlus (AId X) (ANum 1))
+        / empty_state \\ st2,
+
+    where [st2 = { X |-> 1, Y |-> 2 }].  Note that [st1 <> st2]; this
+    is a contradiction, since [ceval] is deterministic!  [] *)
+
+(**Then the next step is to prove this inequiv*)
+
+Theorem subst_inequiv :
+  ~ subst_equiv_property.
+Proof.
+  unfold subst_equiv_property.
+  intros Contra.
+
+  (* Here is the counterexample: assuming that [subst_equiv_property]
+     holds allows us to prove that these two programs are
+     equivalent... *)
+  remember (X ::= APlus (AId X) (ANum 1);;
+            Y ::= AId X)
+      as c1.
+  remember (X ::= APlus (AId X) (ANum 1);;
+            Y ::= APlus (AId X) (ANum 1))
+      as c2.
+  assert (cequiv c1 c2) by (subst; apply Contra).
+
+  (* ... allows us to show that the command [c2] can terminate
+     in two different final states:
+        st1 = {X |-> 1, Y |-> 1}
+        st2 = {X |-> 1, Y |-> 2}. *)
+  remember (t_update (t_update empty_state X 1) Y 1) as st1.
+  remember (t_update (t_update empty_state X 1) Y 2) as st2.
+  assert (H1: c1 / empty_state \\ st1);
+  assert (H2: c2 / empty_state \\ st2);
+  try (subst;
+       apply E_Seq with (st' := (t_update empty_state X 1));
+       apply E_Ass; reflexivity).
+  apply H in H1.
+
+  (* Finally, we use the fact that evaluation is deterministic
+     to obtain a contradiction. *)
+  assert (Hcontra: st1 = st2)
+    by (apply (ceval_deterministic c2 empty_state); assumption).
+  assert (Hcontra': st1 Y = st2 Y)
+    by (rewrite Hcontra; reflexivity).
+  subst. inversion Hcontra'.  Qed.
+
+
+(** Actually, The above equivalence it was actually almost right.  
+    To make it correct, we just need to
+    exclude the case where the variable [X] occurs in the
+    right-hand-side of the first assignment statement. 
+*)
+
+Inductive var_not_used_in_aexp (X:id) : aexp -> Prop :=
+  | VNUNum: forall n, var_not_used_in_aexp X (ANum n)
+  | VNUId: forall Y, X <> Y -> var_not_used_in_aexp X (AId Y)
+  | VNUPlus: forall a1 a2,
+      var_not_used_in_aexp X a1 ->
+      var_not_used_in_aexp X a2 ->
+      var_not_used_in_aexp X (APlus a1 a2)
+  | VNUMinus: forall a1 a2,
+      var_not_used_in_aexp X a1 ->
+      var_not_used_in_aexp X a2 ->
+      var_not_used_in_aexp X (AMinus a1 a2)
+  | VNUMult: forall a1 a2,
+      var_not_used_in_aexp X a1 ->
+      var_not_used_in_aexp X a2 ->
+      var_not_used_in_aexp X (AMult a1 a2).
+
+Lemma aeval_weakening : forall i st a ni,
+  var_not_used_in_aexp i a ->
+  aeval (t_update st i ni) a = aeval st a.
+Proof.
+  intros.
+  induction a; simpl;
+    try (inversion H; subst);
+    try (apply IHa1 in H2; apply IHa2 in H3);
+    try (rewrite H2; rewrite H3);
+    try reflexivity.
+  - (* AId *)
+  apply t_update_neq.
+  assumption.
+Qed.
+
+(** Using var_not_used_in_aexp, we can formalize and prove a correct verson
+    of subst_equiv_property. I call it subst_equiv_weaker_property 
+*)
+
+Lemma aeval__var_not_used_in_aexp: forall a b i st,
+    var_not_used_in_aexp i b ->
+    st i = aeval st b ->
+    aeval st a = aeval st (subst_aexp i b a).
+Proof.
+  induction a; intros;
+    simpl;
+    try rewrite <- IHa1; try rewrite <- IHa2;
+      try destruct (beq_idP i0 i); subst;
+      try reflexivity; try assumption.
+Qed.
+
+Theorem subst_equiv_property_weak: forall i1 i2 a1 a2,
+    var_not_used_in_aexp i1 a1 ->
+    cequiv (i1 ::= a1;; i2 ::= a2)
+           (i1 ::= a1;; i2 ::= subst_aexp i1 a1 a2).
+Proof.
+  intros i1 i2 a1 a2 Hvar.
+  split; intros H; inversion H; subst.
+  - apply E_Seq with st'0.
+    + assumption.
+    + inversion H5; subst. constructor.
+      rewrite <- aeval__var_not_used_in_aexp;
+        try reflexivity; try assumption.
+      * inversion H2; subst.
+        rewrite aeval_weakening; try assumption.
+        unfold t_update. rewrite <- beq_id_refl. reflexivity.
+  - apply E_Seq with st'0.
+    + assumption.
+    + inversion H5; subst. constructor.
+      rewrite <- aeval__var_not_used_in_aexp;
+        try reflexivity; try assumption.
+      * inversion H2; subst.
+        rewrite aeval_weakening; try assumption.
+        unfold t_update. rewrite <- beq_id_refl. reflexivity.
+Qed.
+
+
+(** Here are more example of program inequality.
+    Prove that an infinite loop is not equivalent to [SKIP] 
+*)
+
+Theorem inequiv_exercise:
+  ~ cequiv (WHILE BTrue DO SKIP END) SKIP.
+Proof.
+  unfold not.
+  remember (WHILE BTrue DO SKIP END) as c eqn:Heqc.
+  induction c; try (inversion Heqc).
+  intros.
+  rewrite H1 in *.
+  assert (bequiv b BTrue).
+  unfold bequiv. intros. rewrite H0. simpl. reflexivity.
+  unfold cequiv in H.  
+  apply WHILE_true_nonterm with (c:=SKIP) (st:=empty_state) (st':=empty_state) in H2.
+  unfold not in H2.
+  rewrite H0 in H2.
+  rewrite H in H2.
+  assert (SKIP / empty_state \\ empty_state).
+  apply E_Skip.
+  apply H2 in H3.
+  assumption.
+Qed.  
+
+
+
