final project/README.md
@@ -2,6 +2,24 @@
 Course project for CS386L programming language, using coq language
 Tian Zhang ( tz3272 )
 
-* ConstantFolding.v : implement constant folding for Imp language
-* PartialEvaluation.v : implement partial evaluation on constant folding.
+## Project Introduction
+
+In this final project, I am working in program equivalence, program not equivalence, non-determinitic programming
+and constant folding.
+
+All the work is based on Imp.v and Map.v, and some idea of proof and implementation comes from advanced optional exercise from the software foundation book.
+
+I planed to implement partial evaluation, however, all the detail are in PE.v file in the book. As a result, I just read and learn that
+chapter, and do not implement my own version.
+
+
+
+## Project Detail
+-----------------------------
+* programEquivalence.v : define program equivalence and its properities, starting point of the project.
+* forWhileEquiv.v : Idea comes from Midterm, prove that for and while loop are equivalent.
+* programNotEquivalence.v : define and prove that program are not equivalent. Analysis arithmetic expression substitution.
+* NonDeterministic.v : introduce Havoc, a non-deterministic command, and prove its behaviour equivalence. 
+* ConstantFolding.v : implement constant folding for Imp language, and proof its correctness
+* PartialEvaluation.v :  partial evaluation , same as PE.v, no my work in this file.
 
